Some preliminaries for indirect offsets

src/Dafny/examples/fs/indirect_fs.dfy
@@ -11,7 +11,149 @@ module IndFs
   import opened Fs
   import opened Marshal
   import opened IndBlocks
+  import opened Pow
   import C = Collections
+
+  datatype preIndOff = IndOff(ilevel: nat, j: nat)
+  {
+    static const direct: IndOff := IndOff(0, 0)
+    // if this is true then this IndOff points directly to data
+    const data?: bool := ilevel == 0
+
+    predicate Valid()
+    {
+      j < pow(512, ilevel)
+    }
+
+    // to dereference an offset, we can decompose it into a single indirection
+    // then the remaining lookup at one level lower
+    function split(): (p: (IndOff, IndOff))
+      requires Valid()
+      requires ilevel > 0
+    {
+      Arith.div_positive_auto();
+      var k := pow(512, ilevel-1);
+      Arith.div_mod_split(j, k);
+      assert pow(512, ilevel) == k * 512;
+      Arith.div_incr_auto();
+      (IndOff(1, j / k), IndOff(ilevel-1, j % k))
+    }
+  }
+  type IndOff = x:preIndOff | x.Valid() witness IndOff(0, 0)
+
+  datatype Config = Config(ilevels: seq<nat>)
+  {
+    const totals := configSum(ilevels)
+    const total := configTotal(ilevels)
+
+    static function method configTotal(ilevels: seq<nat>): nat
+    {
+      if ilevels == [] then 0
+      else pow(512, ilevels[0]) + configTotal(ilevels[1..])
+    }
+
+    static lemma test_configSum1()
+      ensures configSum([0]) == [0,1]
+    {}
+
+    static lemma test_configSum2()
+      ensures configSum([0,1]) == [0,1,1+512]
+    {
+      assert [0,1][..1] == [0];
+    }
+
+    static lemma test_configSum3()
+      ensures configSum([0,0,1,2]) == [0,1,2,2+512, 2+512+512*512]
+    {
+      assert configTotal([0,0,1,2]) == 2+512+512*512;
+      assert [0,0,1,2][..3] == [0,0,1];
+      assert [0,0,1][..2] == [0,0];
+      assert [0,0][..1] == [0];
+    }
+
+    static function method configSum(ilevels: seq<nat>): (s:seq<nat>)
+      ensures |s| == 1+|ilevels|
+      ensures forall i | 0 <= i <= |ilevels| :: s[i] == configTotal(ilevels[..i])
+    {
+      if ilevels == [] then [0]
+      else (
+        assert ilevels[..|ilevels|] == ilevels;
+        var s := configSum(ilevels[..|ilevels|-1]) + [configTotal(ilevels)];
+        assert s[|ilevels|] == configTotal(ilevels);
+        // NOTE(tej): need to assert this to get into statement context; see
+        // https://dafny-lang.github.io/dafny/DafnyRef/DafnyRef#2036-statements-in-an-expression
+        // which does not include forall statements
+        assert forall i | 0 <= i <= |ilevels| :: s[i] == configTotal(ilevels[..i]) by
+        {
+          forall i | 0 <= i <= |ilevels|
+            ensures s[i] == configTotal(ilevels[..i])
+          {
+            if i == |ilevels| {}
+            else {
+              calc {
+                s[i];
+                configSum(ilevels[..|ilevels|-1])[i];
+                { assert ilevels[..|ilevels|-1][..i] == ilevels[..i]; }
+                configTotal(ilevels[..i]);
+              }
+            }
+          }
+        }
+        s
+      )
+    }
+
+  }
+
+  const config: Config := Config([0,0,0,0,0,0,0,0,0,0,1,1,1,1,3])
+
+  lemma config_properties()
+    ensures |config.ilevels| == 15
+    ensures config.total == 10 + 4*512 + 512*512*512
+    // these inodes can hold at least 10GB
+    ensures config.total * 4 / 1024 /* MB */ > 10_000
+  {}
+
+  datatype preIdx = Idx(k: nat, off: IndOff)
+  {
+    function data?(): bool
+      requires Valid()
+    {
+      off.ilevel == config.ilevels[k]
+    }
+
+    predicate Valid()
+    {
+      && k < |config.ilevels|
+      && off.ilevel <= config.ilevels[k]
+    }
+
+    function flat(): nat
+      requires Valid()
+      requires this.data?()
+    {
+      config.totals[k] + off.j
+    }
+
+    static function from_flat(n: nat): (i:Idx)
+      requires n < config.total
+      ensures i.data?()
+    {
+      if n < 10 then
+        Idx(n, IndOff.direct)
+      else (
+        var n: nat := n-10;
+        if n < 4*512 then
+          Idx(10+n/512, IndOff(1, n%512))
+        else (
+          var n: nat := n-4*512;
+          Idx(14, IndOff(3, n%(512*512*512)))
+        )
+      )
+    }
+
+  }
+  type Idx = x:preIdx | x.Valid() witness Idx(0, IndOff(0, 0))
 
   class IndFilesys
   {
